WSTuple.delete

Bedrock/Platform/Facade/examples/WSTuple.v
@@ -3,9 +3,14 @@ Require Import Bedrock.Platform.Malloc Bedrock.Platform.Arrays8.
 Require Import Bedrock.Platform.Facade.examples.ByteString.
 
 
+Inductive nonempty (ws : WSTupl) : Prop :=
+| Nonempty : forall len : W, len <> $0 -> wordToNat len = length ws -> nonempty ws.
+Hint Constructors nonempty.
+
 Module Type ADT.
   Parameter wstuple : WSTupl -> W -> HProp.
   Parameter wstuple' : WSTupl -> W -> HProp.
+  Parameter wsitem : WS -> W -> W -> HProp.
 
   Axiom wstuple_fwd : forall ws p, wstuple ws p ===> wstuple' ws p * [| p <> 0 |] * [| freeable p (length ws * 2) |].
   Axiom wstuple_bwd : forall ws p, wstuple' ws p * [| p <> 0 |] * [| freeable p (length ws * 2) |] ===> wstuple ws p.
@@ -13,6 +18,17 @@ Module Type ADT.
   Axiom wstuple'_nil_fwd : forall p, wstuple' nil p ===> Emp.
   Axiom wstuple'_word_fwd : forall w ws' p, wstuple' (WSWord w :: ws') p ===> (p ==*> $0, w) * wstuple' ws' (p ^+ $8).
   Axiom wstuple'_bytes_fwd : forall capacity bs ws' p, wstuple' (WSBytes capacity bs :: ws') p ===> Ex sp, (p ==*> $1, sp) * bytes capacity bs sp * wstuple' ws' (p ^+ $8).
+
+  Axiom wstuple'_nonzero_fwd : forall ws p,
+      nonempty ws
+      -> wstuple' ws p ===> Ex w, Ex ws', Ex tag, Ex sp,
+           [| ws = w :: ws' |] * (p ==*> tag, sp) * wsitem w tag sp * wstuple' ws' (p ^+ $8).
+  Axiom wsitem_word_fwd : forall w tag sp,
+      tag = $0
+      -> wsitem w tag sp ===> [| w = WSWord sp |].
+  Axiom wsitem_bytes_fwd : forall w tag sp,
+      tag <> $0
+      -> wsitem w tag sp ===> Ex capacity, Ex bs, [| w = WSBytes capacity bs |] * bytes capacity bs sp.
 
   Axiom wstuple'_nil_bwd : forall p, Emp ===> wstuple' nil p.
   Axiom wstuple'_word_bwd : forall w ws' p, (p ==*> $0, w) * wstuple' ws' (p ^+ $8) ===> wstuple' (WSWord w :: ws') p.
@@ -32,6 +48,12 @@ Module Import Adt : ADT.
   Definition wstuple (ws : WSTupl) (p : W) : HProp :=
     wstuple' ws p * [| p <> 0 |] * [| freeable p (length ws * 2) |].
 
+  Definition wsitem (w : WS) (tag p : W) :=
+    match w with
+    | WSWord w => [| tag = $0 |] * [| w = p |]
+    | WSBytes capacity bs => [| tag = $1 |] * bytes capacity bs p
+    end.
+
   Theorem wstuple_fwd : forall ws p, wstuple ws p ===> wstuple' ws p * [| p <> 0 |] * [| freeable p (length ws * 2) |].
   Proof.
     unfold wstuple; sepLemma.
@@ -50,6 +72,39 @@ Module Import Adt : ADT.
   Theorem wstuple'_word_fwd : forall w ws' p, wstuple' (WSWord w :: ws') p ===> (p ==*> $0, w) * wstuple' ws' (p ^+ $8).
   Proof.
     sepLemma.
+  Qed.
+
+  Theorem wstuple'_nonzero_fwd : forall ws p,
+      nonempty ws
+      -> wstuple' ws p ===> Ex w, Ex ws', Ex tag, Ex sp,
+           [| ws = w :: ws' |] * (p ==*> tag, sp) * wsitem w tag sp * wstuple' ws' (p ^+ $8).
+  Proof.
+    destruct 1.
+    destruct ws; simpl; intuition.
+    apply (f_equal (natToWord 32)) in H0.
+    rewrite natToWord_wordToNat in H0.
+    tauto.
+    destruct w.
+    sepLemma.
+    simpl.
+    sepLemma.
+    sepLemma.
+    simpl.
+    sepLemma.
+  Qed.
+
+  Theorem wsitem_word_fwd : forall w tag sp,
+      tag = $0
+      -> wsitem w tag sp ===> [| w = WSWord sp |].
+  Proof.
+    destruct w; sepLemma; discriminate.
+  Qed.
+
+  Theorem wsitem_bytes_fwd : forall w tag sp,
+      tag <> $0
+      -> wsitem w tag sp ===> Ex capacity, Ex bs, [| w = WSBytes capacity bs |] * bytes capacity bs sp.
+  Proof.
+    destruct w; sepLemma; discriminate.
   Qed.
 
   Theorem wstuple'_bytes_fwd : forall capacity bs ws' p, wstuple' (WSBytes capacity bs :: ws') p ===> Ex sp, (p ==*> $1, sp) * bytes capacity bs sp * wstuple' ws' (p ^+ $8).
@@ -127,20 +182,85 @@ Proof.
   omega.
 Qed.
 
+Lemma allocated2 : forall base offset,
+    (Ex v1, Ex v2, (base ^+ $ offset) =*> v1 * (base ^+ ($ offset ^+ $4)) =*> v2) ===> allocated base offset 2.
+Proof.
+  simpl.
+  destruct offset; sepLemma.
+  replace (S (S (S (S (S offset))))) with (S offset + 4) by omega.
+  sepLemma.
+Qed.
+
+Lemma wtimes8 : forall n,
+      natToW (n * 8) = natToW n ^* $8.
+Proof.
+  intros.
+  replace (n * 8) with (8 * n) by omega.
+  simpl.
+  repeat rewrite natToW_plus.
+  words.
+Qed.
+
+Opaque mult.
+
+Lemma blob_absorb : forall (len tmpl self : W),
+    (wordToNat len >= wordToNat tmpl)%nat
+    -> tmpl <> $0
+    -> (Ex v1, Ex v2, self =?> ((wordToNat len - wordToNat tmpl) * 2) * (self ^+ (len ^- tmpl) ^* $8) =*> v1 * (self ^+ (len ^- tmpl) ^* $8 ^+ $4) =*> v2)
+    ===> self =?> ((wordToNat len - (wordToNat tmpl - 1)) * 2).
+Proof.
+  intros.
+  eapply Himp_trans; [ | apply allocated_join with (len' := (wordToNat len - wordToNat tmpl) * 2) ].
+  replace ((wordToNat len - (wordToNat tmpl - 1)) * 2 -
+           (wordToNat len - wordToNat tmpl) * 2) with 2.
+  eapply Himp_trans; [ | apply Himp_star_frame; [ apply Himp_refl | apply allocated2 ] ].
+  sepLemma.
+  replace (4 * ((wordToNat len - wordToNat tmpl) * 2))
+          with ((wordToNat len - wordToNat tmpl) * 8) by omega.
+  rewrite natToW_plus.
+  rewrite <- wordToNat_wminus by nomega.
+  rewrite wtimes8.
+  unfold natToW.
+  rewrite natToWord_wordToNat.
+  replace (self ^+ ((len ^- tmpl) ^* $ (8) ^+ $ (4)))
+    with (self ^+ (len ^- tmpl) ^* $ (8) ^+ $ (4)) by words.
+  sepLemma.
+  assert (wordToNat tmpl <> 0).
+  intro.
+  apply (f_equal (natToWord 32)) in H1.
+  rewrite natToWord_wordToNat in H1.
+  tauto.
+  omega.
+  pre_nomega.
+  change (wordToNat $1) with 1.
+  case_eq (wordToNat tmpl); intros.
+  apply (f_equal (natToWord 32)) in H1.
+  rewrite natToWord_wordToNat in H1.
+  tauto.    
+  omega.
+Qed.
+
 Definition hints : TacPackage.
   prepare (wstuple_fwd, wstuple'_nil_fwd, wstuple'_word_fwd, wstuple'_bytes_fwd,
-           expose_words)
+           expose_words, wstuple'_nonzero_fwd, wsitem_word_fwd, wsitem_bytes_fwd)
           (wstuple_bwd, wstuple'_nil_bwd, wstuple'_word_bwd, wstuple'_bytes_bwd,
-           zeroes_nonzero_bwd).
+           zeroes_nonzero_bwd, blob_absorb).
 Defined.
 
 Definition newS := SPEC("extra_stack", "len") reserving 8
   PRE[V] [| wordToNat (V "len") >= 1 |]%nat * [| goodSize (wordToNat (V "len") * 2) |] * mallocHeap 0
   POST[R] wstuple (zeroes (wordToNat (V "len"))) R * mallocHeap 0.
 
-Definition m := bimport [[ "malloc"!"malloc" @ [mallocS], "malloc"!"free" @ [freeS] ]]
+Definition deleteS := SPEC("extra_stack", "self", "len") reserving 11
+  Al ws,
+  PRE[V] wstuple ws (V "self") * [| wordToNat (V "len") = length ws |] * mallocHeap 0
+  POST[R] [| R = $0 |] * mallocHeap 0.
+
+Definition m := bimport [[ "malloc"!"malloc" @ [mallocS], "malloc"!"free" @ [freeS],
+                           "ByteString"!"delete" @ [ByteString.deleteS],
+                           "ByteString"!"copy" @ [ByteString.copyS] ]]
   bmodule "WSTuple" {{
-    bfunction "new"("extra_stack", "len", "tmp") [newS]
+    (*bfunction "new"("extra_stack", "len", "tmp") [newS]
       "extra_stack" <- "len" * 2;;
       "extra_stack" <-- Call "malloc"!"malloc"(0, "extra_stack")
       [PRE[V, R] R =?> (wordToNat (V "len") * 2) * [| goodSize (wordToNat (V "len") * 2) |]
@@ -157,6 +277,57 @@ Definition m := bimport [[ "malloc"!"malloc" @ [mallocS], "malloc"!"free" @ [fre
       };;
 
       Return "extra_stack"
+    end
+
+    with*) bfunction "delete"("extra_stack", "self", "len", "tmp", "tmpl") [deleteS]
+      "tmp" <- "self";;
+      "tmpl" <- "len";;
+      [Al ws,
+       PRE[V] wstuple' ws (V "tmp")
+              * [| wordToNat (V "tmpl") = length ws |]
+              * V "self" =?> ((wordToNat (V "len") - wordToNat (V "tmpl")) * 2)
+              * [| wordToNat (V "len") >= wordToNat (V "tmpl") |]%nat
+              * [| V "tmp" = V "self" ^+ ((V "len" ^- V "tmpl") ^* $8) |]
+              * [| V "self" <> $0 |] * [| freeable (V "self") (wordToNat (V "len") * 2) |]
+              * mallocHeap 0
+       POST[R] [| R = $0 |] * mallocHeap 0 ]
+      While ("tmpl" <> 0) {
+        Assert [Al ws,
+                PRE[V] wstuple' ws (V "tmp")
+                       * [| wordToNat (V "tmpl") = length ws |]
+                       * V "self" =?> ((wordToNat (V "len") - wordToNat (V "tmpl")) * 2)
+                       * [| wordToNat (V "len") >= wordToNat (V "tmpl") |]%nat
+                       * [| V "tmp" = V "self" ^+ ((V "len" ^- V "tmpl") ^* $8) |]
+                       * [| V "self" <> $0 |] * [| freeable (V "self") (wordToNat (V "len") * 2) |]
+                       * [| nonempty ws |] * [| V "tmpl" <> 0 |]
+                       * mallocHeap 0
+                POST[R] [| R = $0 |] * mallocHeap 0 ];;
+
+        "extra_stack" <-* "tmp";;
+        If ("extra_stack" = 0) {
+          Skip
+        } else {
+          "extra_stack" <-* "tmp"+4;;
+          Call "ByteString"!"delete"("extra_stack", "extra_stack")
+          [Al ws,
+           PRE[V] wstuple' ws (V "tmp" ^+ $8)
+                  * [| wordToNat (V "tmpl" ^- $1) = length ws |]
+                  * V "self" =?> ((wordToNat (V "len") - wordToNat (V "tmpl" ^- $1)) * 2)
+                  * [| wordToNat (V "len") >= wordToNat (V "tmpl" ^- $1) |]%nat
+                  * [| V "tmp" ^+ $8 = V "self" ^+ ((V "len" ^- (V "tmpl" ^- $1)) ^* $8) |]
+                  * [| V "self" <> $0 |] * [| freeable (V "self") (wordToNat (V "len") * 2) |]
+                  * mallocHeap 0
+           POST[R] [| R = $0 |] * mallocHeap 0 ]
+         };;
+        "tmp" <- "tmp" + 8;;
+        "tmpl" <- "tmpl" - 1
+      };;
+
+      "len" <- "len" * 2;;
+      Call "malloc"!"free"(0, "self", "len")
+      [PRE[_] Emp
+       POST[R] [| R = $0 |] ];;
+      Return 0
     end
   }}.
 
@@ -226,15 +397,183 @@ Qed.
 
 Hint Extern 1 (himp _ _ _) => apply zeroes_zero_bwd.
 
-Ltac t := sep hints; auto.
+Lemma goodlength_godown : forall (w : W) n,
+    wordToNat w = S n
+    -> wordToNat (w ^- $1) = n.
+Proof.
+  intros.
+  rewrite wordToNat_wminus.
+  change (wordToNat $1) with 1.
+  omega.
+  pre_nomega.
+  change (wordToNat $1) with 1.
+  omega.
+Qed.
+
+Hint Immediate goodlength_godown.
+
+Lemma geq_godown : forall len (tmpl : W) n,
+    (len >= wordToNat tmpl)%nat
+    -> wordToNat tmpl = S n
+    -> (len >= wordToNat (tmpl ^- $1))%nat.
+Proof.
+  intros.
+  rewrite H0 in *.
+  rewrite wordToNat_wminus.
+  change (wordToNat $1) with 1.
+  omega.
+  pre_nomega.
+  change (wordToNat $1) with 1.
+  omega.
+Qed.
+
+Hint Immediate geq_godown.
+
+Hint Extern 1 (?x ^+ _ = _) =>
+  match goal with
+  | [ H : x = _ |- _ ] => rewrite H; words
+  end.
+
+Lemma minus_positive : forall w : W,
+    w <> $0
+    -> wordToNat (w ^- $1) = wordToNat w - 1.
+Proof.
+  intros; rewrite wordToNat_wminus; auto.
+  pre_nomega.
+  change (wordToNat $1) with 1.
+  case_eq (wordToNat w); intros.
+  apply (f_equal (natToWord 32)) in H0.
+  rewrite natToWord_wordToNat in H0.
+  tauto.
+  omega.
+Qed.
+
+Hint Rewrite minus_positive using assumption : sepFormula.
+
+Inductive containsAllocated : HProp -> nat -> Prop :=
+| CAlBase : forall len p, containsAllocated (p =?> len)%Sep len
+| CAlLeft : forall P Q len, containsAllocated P len
+  -> containsAllocated (SEP.ST.star P Q) len
+| CAlRight : forall P Q len, containsAllocated Q len
+  -> containsAllocated (SEP.ST.star P Q) len.
+
+Hint Constructors containsAllocated.
+
+Require Import Bedrock.Platform.MoreArrays.
+
+Lemma containsAllocated_containsArray : forall P len,
+    containsAllocated P len
+    -> exists Q, P ===> Ex ws, Ex p, array ws p * [| length ws = len |] * Q.
+Proof.
+  induction 1.
+
+  exists Emp%Sep.
+  eapply Himp_trans; [ apply allocate_array; auto | ].
+  sepLemma.
+
+  destruct IHcontainsAllocated.
+  exists (x * Q)%Sep.
+  eapply Himp_trans; [ eapply Himp_star_frame; [ apply H0 | apply Himp_refl ] | ].
+  clear H.
+  sepLemma.
+
+  destruct IHcontainsAllocated.
+  exists (x * P)%Sep.
+  eapply Himp_trans; [ eapply Himp_star_frame; [ apply Himp_refl | apply H0 ] | ].
+  clear H.
+  sepLemma.
+Qed.
+
+Lemma use_Himp : forall cs P arg P',
+    interp cs (![P] arg)
+    -> P ===> P'
+    -> interp cs (![P'] arg).
+Proof.
+  intros.
+  rewrite sepFormula_eq in *.
+  destruct arg.
+  unfold Himp, himp in H0.
+  eapply Imply_E.
+  apply H0.
+  assumption.
+Qed.
+
+Theorem containsAllocated_goodSize : forall cs P stn st len,
+    interp cs (![P] (stn, st))
+    -> containsAllocated P len
+    -> goodSize len.
+Proof.
+  intros.
+  apply containsAllocated_containsArray in H0.
+  destruct H0.
+  eapply use_Himp in H0; eauto.
+  evaluate auto_ext.
+  fold (@length W) in *.
+  subst.
+  eapply containsArray_goodSize; eauto.
+Qed.
+
+Hint Rewrite times2
+     using eapply goodSize_weaken; [ eapply containsAllocated_goodSize; [ eassumption | eauto ] | match goal with
+                                                                                                  | [ H : _ = natToW 0 |- _ ] => rewrite H; change (wordToNat (natToW 0)) with 0; omega
+                                                                                                  end ] : sepFormula.
+
+Lemma tmpl_zero : forall tmpl n,
+    tmpl = natToW 0
+    -> n - wordToNat tmpl = n.
+Proof.
+  intros; subst.
+  change (wordToNat (natToW 0)) with 0.
+  omega.
+Qed.
+
+Hint Rewrite tmpl_zero using assumption : sepFormula.
+
+Lemma wstuple_delete : forall specs ws tmp tmpl,
+    wordToNat tmpl = length ws
+    -> tmpl = natToW 0
+    -> himp specs (wstuple' ws tmp) (SEP.ST.emp W (settings * state)).
+Proof.
+  intros; subst.
+  change (wordToNat (natToW 0)) with 0 in *.
+  destruct ws; simpl in *; try discriminate.
+  step hints.
+Qed.
+
+Hint Extern 1 (himp _ (wstuple' _ _) _ ) => eapply wstuple_delete; eassumption.
+
+Ltac t := solve [ sep hints; eauto ].
 
 Local Hint Extern 1 (@eq W _ _) => words.
 Local Hint Extern 1 (freeable _ _) => congruence.
+Hint Rewrite Minus.minus_diag : sepFormula.
+
+Transparent mult.
 
 Theorem ok : moduleOk m.
 Proof.
   vcgen.
 
+  (*t.
+  t.
+  t.
+  t.
+  t.
+  t.
+  t.
+  t.
+  t.
+  t.
+  t.
+  t.
+  t.*)
+
+  t.
+  t.
+  t.
+  t.
+  t.
+  t.
   t.
   t.
   t.
